gravy/test/out2.bpl
@@ -187,3 +187,489 @@ var temp$47 : int;
     return;
 }
 
+
+implementation int$InfeasibleCode01$infeasible0$1890($this:ref, $in_parameter__0:ref) returns ($return:int, $exception:ref){
+    
+var temp$015 : ref;    
+var temp$419 : int;    
+var arr13 : ref;    
+var temp$217 : int;    
+var temp$116 : int;    
+var i14 : int;    
+var this12 : ref;    
+var temp$520 : int;    
+var temp$318 : ref;
+    assume { :sourceloc "/Users/schaef/git/jar2bpl/jar2bpl_test/regression/true_positives/tp01/InfeasibleCode01.java",-1,-1,-1,-1 } $this != $null;
+    assert { :sourceloc "/Users/schaef/git/jar2bpl/jar2bpl_test/regression/true_positives/tp01/InfeasibleCode01.java",27,2,31,2 } true;
+    this12 := $this;
+    assert { :sourceloc "/Users/schaef/git/jar2bpl/jar2bpl_test/regression/true_positives/tp01/InfeasibleCode01.java",27,25,27,33 } true;
+    arr13 := $in_parameter__0;
+    assert { :sourceloc "/Users/schaef/git/jar2bpl/jar2bpl_test/regression/true_positives/tp01/InfeasibleCode01.java",28,3,28,21 } true;
+    assert { :sourceloc "/Users/schaef/git/jar2bpl/jar2bpl_test/regression/true_positives/tp01/InfeasibleCode01.java",28,3,28,21 } arr13 != $null;
+    i14 := $arrSizeHeap[arr13];
+    assert { :sourceloc "/Users/schaef/git/jar2bpl/jar2bpl_test/regression/true_positives/tp01/InfeasibleCode01.java",29,3,29,11 } true;
+    temp$015 := arr13;
+    assert { :sourceloc "/Users/schaef/git/jar2bpl/jar2bpl_test/regression/true_positives/tp01/InfeasibleCode01.java",29,3,29,11 } true;
+    temp$116 := 3;
+    assert { :sourceloc "/Users/schaef/git/jar2bpl/jar2bpl_test/regression/true_positives/tp01/InfeasibleCode01.java",29,6,29,8 } true;
+    temp$217 := 3;
+    assert { :sourceloc "/Users/schaef/git/jar2bpl/jar2bpl_test/regression/true_positives/tp01/InfeasibleCode01.java",29,6,29,8 } true;
+    assert { :sourceloc "/Users/schaef/git/jar2bpl/jar2bpl_test/regression/true_positives/tp01/InfeasibleCode01.java",29,6,29,8 } temp$116 < $arrSizeHeap[temp$015] && temp$116 >= 0;
+    $intArrHeap := $intArrHeap[temp$015 := $intArrHeap[temp$015][temp$116 := temp$217]];
+    assert { :sourceloc "/Users/schaef/git/jar2bpl/jar2bpl_test/regression/true_positives/tp01/InfeasibleCode01.java",29,6,29,8 } true;
+    temp$318 := arr13;
+    assert { :sourceloc "/Users/schaef/git/jar2bpl/jar2bpl_test/regression/true_positives/tp01/InfeasibleCode01.java",29,6,29,8 } true;
+    temp$419 := i14;
+    assert { :sourceloc "/Users/schaef/git/jar2bpl/jar2bpl_test/regression/true_positives/tp01/InfeasibleCode01.java",29,6,29,8 } true;
+    assert { :sourceloc "/Users/schaef/git/jar2bpl/jar2bpl_test/regression/true_positives/tp01/InfeasibleCode01.java",29,6,29,8 } temp$419 < $arrSizeHeap[temp$318] && temp$419 >= 0;
+    temp$520 := $intArrHeap[temp$318][temp$419];
+    assert { :sourceloc "/Users/schaef/git/jar2bpl/jar2bpl_test/regression/true_positives/tp01/InfeasibleCode01.java",30,3,30,16 } true;
+    $return := temp$520;
+    return;
+}
+
+
+implementation int$InfeasibleCode01$infeasible1$1891($this:ref, $in_parameter__0:ref) returns ($return:int, $exception:ref){
+    
+var this21 : ref;    
+var temp$528 : int;    
+var temp$124 : ref;    
+var $fakelocal_0 : ref;    
+var temp$023 : int;    
+var $fakelocal_2 : ref;    
+var $fakelocal_1 : ref;    
+var temp$225 : ref;    
+var temp$326 : ref;    
+var temp$427 : ref;    
+var o22 : ref;
+    assume { :sourceloc "/Users/schaef/git/jar2bpl/jar2bpl_test/regression/true_positives/tp01/InfeasibleCode01.java",-1,-1,-1,-1 } $this != $null;
+    assume $heap[$in_parameter__0,$type] <: java.lang.Object;
+    assert { :sourceloc "/Users/schaef/git/jar2bpl/jar2bpl_test/regression/true_positives/tp01/InfeasibleCode01.java",33,2,39,2 } true;
+    this21 := $this;
+    assert { :sourceloc "/Users/schaef/git/jar2bpl/jar2bpl_test/regression/true_positives/tp01/InfeasibleCode01.java",33,25,33,32 } true;
+    o22 := $in_parameter__0;
+    assert { :sourceloc "/Users/schaef/git/jar2bpl/jar2bpl_test/regression/true_positives/tp01/InfeasibleCode01.java",34,7,34,13 } true;
+    if (o22 != $null) {
+        assert { :sourceloc "/Users/schaef/git/jar2bpl/jar2bpl_test/regression/true_positives/tp01/InfeasibleCode01.java",34,7,34,13 } { :comment "thenblock" } true;
+        goto block7;
+    } else {
+        assert { :sourceloc "/Users/schaef/git/jar2bpl/jar2bpl_test/regression/true_positives/tp01/InfeasibleCode01.java",34,7,34,13 } { :comment "elseblock" } true;
+    }
+    assert { :sourceloc "/Users/schaef/git/jar2bpl/jar2bpl_test/regression/true_positives/tp01/InfeasibleCode01.java",34,7,34,13 } true;
+    goto block8;
+  block7:
+    assert { :sourceloc "/Users/schaef/git/jar2bpl/jar2bpl_test/regression/true_positives/tp01/InfeasibleCode01.java",34,7,34,13 } true;
+    assert { :sourceloc "/Users/schaef/git/jar2bpl/jar2bpl_test/regression/true_positives/tp01/InfeasibleCode01.java",34,7,34,13 } true;
+    call temp$023, $exception := int$java.lang.Object$hashCode$41(o22);
+    assert { :sourceloc "/Users/schaef/git/jar2bpl/jar2bpl_test/regression/true_positives/tp01/InfeasibleCode01.java",35,4,35,23 } true;
+    $return := temp$023;
+    return;
+  block8:
+    assert { :sourceloc "/Users/schaef/git/jar2bpl/jar2bpl_test/regression/true_positives/tp01/InfeasibleCode01.java",35,4,35,23 } true;
+    assert { :sourceloc "/Users/schaef/git/jar2bpl/jar2bpl_test/regression/true_positives/tp01/InfeasibleCode01.java",37,3,37,55 } true;
+    temp$124 := java.io.PrintStream$java.lang.System$err237;
+    assert { :sourceloc "/Users/schaef/git/jar2bpl/jar2bpl_test/regression/true_positives/tp01/InfeasibleCode01.java",37,3,37,55 } true;
+    call $fakelocal_0 := $new(java.lang.StringBuffer);
+    temp$225 := $fakelocal_0;
+    assert { :sourceloc "/Users/schaef/git/jar2bpl/jar2bpl_test/regression/true_positives/tp01/InfeasibleCode01.java",37,22,37,53 } true;
+    call $exception := void$java.lang.StringBuffer$$la$init$ra$$685(temp$225);
+    assert { :sourceloc "/Users/schaef/git/jar2bpl/jar2bpl_test/regression/true_positives/tp01/InfeasibleCode01.java",37,22,37,53 } true;
+    assert { :sourceloc "/Users/schaef/git/jar2bpl/jar2bpl_test/regression/true_positives/tp01/InfeasibleCode01.java",37,22,37,53 } o22 != $null;
+    call temp$326, $exception := java.lang.String$java.lang.Object$toString$44(o22);
+    assert { :sourceloc "/Users/schaef/git/jar2bpl/jar2bpl_test/regression/true_positives/tp01/InfeasibleCode01.java",37,22,37,53 } true;
+    call $fakelocal_1, $exception := java.lang.StringBuffer$java.lang.StringBuffer$append$701(temp$225, temp$326);
+    assert { :sourceloc "/Users/schaef/git/jar2bpl/jar2bpl_test/regression/true_positives/tp01/InfeasibleCode01.java",37,22,37,53 } true;
+    call $fakelocal_2, $exception := java.lang.StringBuffer$java.lang.StringBuffer$append$701(temp$225, $StringConst0);
+    assert { :sourceloc "/Users/schaef/git/jar2bpl/jar2bpl_test/regression/true_positives/tp01/InfeasibleCode01.java",37,22,37,53 } true;
+    call temp$427, $exception := java.lang.String$java.lang.StringBuffer$toString$738(temp$225);
+    assert { :sourceloc "/Users/schaef/git/jar2bpl/jar2bpl_test/regression/true_positives/tp01/InfeasibleCode01.java",37,22,37,53 } true;
+    assert { :sourceloc "/Users/schaef/git/jar2bpl/jar2bpl_test/regression/true_positives/tp01/InfeasibleCode01.java",37,22,37,53 } temp$124 != $null;
+    call $exception := void$java.io.PrintStream$println$217(temp$124, temp$427);
+    assert { :sourceloc "/Users/schaef/git/jar2bpl/jar2bpl_test/regression/true_positives/tp01/InfeasibleCode01.java",37,22,37,53 } true;
+    temp$528 := 2;
+    assert { :sourceloc "/Users/schaef/git/jar2bpl/jar2bpl_test/regression/true_positives/tp01/InfeasibleCode01.java",38,3,38,11 } true;
+    $return := temp$528;
+    return;
+}
+
+
+implementation void$InfeasibleCode01$infeasible2$1892($this:ref, $in_parameter__0:ref) returns ($exception:ref){
+    
+var temp$335 : int;    
+var this29 : ref;    
+var temp$436 : int;    
+var temp$032 : int;    
+var temp$133 : ref;    
+var temp$234 : int;    
+var i31 : int;    
+var arr30 : ref;
+    assume { :sourceloc "/Users/schaef/git/jar2bpl/jar2bpl_test/regression/true_positives/tp01/InfeasibleCode01.java",-1,-1,-1,-1 } $this != $null;
+    assert { :sourceloc "/Users/schaef/git/jar2bpl/jar2bpl_test/regression/true_positives/tp01/InfeasibleCode01.java",41,2,45,2 } true;
+    this29 := $this;
+    assert { :sourceloc "/Users/schaef/git/jar2bpl/jar2bpl_test/regression/true_positives/tp01/InfeasibleCode01.java",41,26,41,35 } true;
+    arr30 := $in_parameter__0;
+    assert { :sourceloc "/Users/schaef/git/jar2bpl/jar2bpl_test/regression/true_positives/tp01/InfeasibleCode01.java",42,8,42,14 } true;
+    i31 := 0;
+  block9:
+    assert { :sourceloc "/Users/schaef/git/jar2bpl/jar2bpl_test/regression/true_positives/tp01/InfeasibleCode01.java",42,8,42,14 } true;
+    assert { :sourceloc "/Users/schaef/git/jar2bpl/jar2bpl_test/regression/true_positives/tp01/InfeasibleCode01.java",42,17,42,29 } true;
+    assert { :sourceloc "/Users/schaef/git/jar2bpl/jar2bpl_test/regression/true_positives/tp01/InfeasibleCode01.java",42,17,42,29 } arr30 != $null;
+    temp$032 := $arrSizeHeap[arr30];
+    assert { :sourceloc "/Users/schaef/git/jar2bpl/jar2bpl_test/regression/true_positives/tp01/InfeasibleCode01.java",42,17,42,29 } true;
+    if (i31 <= temp$032) {
+        assert { :sourceloc "/Users/schaef/git/jar2bpl/jar2bpl_test/regression/true_positives/tp01/InfeasibleCode01.java",42,17,42,29 } { :comment "thenblock" } true;
+        goto block10;
+    } else {
+        assert { :sourceloc "/Users/schaef/git/jar2bpl/jar2bpl_test/regression/true_positives/tp01/InfeasibleCode01.java",42,17,42,29 } { :comment "elseblock" } true;
+    }
+    assert { :sourceloc "/Users/schaef/git/jar2bpl/jar2bpl_test/regression/true_positives/tp01/InfeasibleCode01.java",42,17,42,29 } true;
+    goto block11;
+  block10:
+    assert { :sourceloc "/Users/schaef/git/jar2bpl/jar2bpl_test/regression/true_positives/tp01/InfeasibleCode01.java",42,17,42,29 } true;
+    assert { :sourceloc "/Users/schaef/git/jar2bpl/jar2bpl_test/regression/true_positives/tp01/InfeasibleCode01.java",43,4,43,12 } true;
+    temp$133 := arr30;
+    assert { :sourceloc "/Users/schaef/git/jar2bpl/jar2bpl_test/regression/true_positives/tp01/InfeasibleCode01.java",43,4,43,12 } true;
+    temp$234 := i31;
+    assert { :sourceloc "/Users/schaef/git/jar2bpl/jar2bpl_test/regression/true_positives/tp01/InfeasibleCode01.java",43,7,43,9 } true;
+    assert { :sourceloc "/Users/schaef/git/jar2bpl/jar2bpl_test/regression/true_positives/tp01/InfeasibleCode01.java",43,7,43,9 } temp$234 < $arrSizeHeap[temp$133] && temp$234 >= 0;
+    $intArrHeap := $intArrHeap[temp$133 := $intArrHeap[temp$133][temp$234 := i31]];
+    assert { :sourceloc "/Users/schaef/git/jar2bpl/jar2bpl_test/regression/true_positives/tp01/InfeasibleCode01.java",43,7,43,9 } true;
+    assert { :sourceloc "/Users/schaef/git/jar2bpl/jar2bpl_test/regression/true_positives/tp01/InfeasibleCode01.java",42,31,42,33 } true;
+    temp$335 := i31;
+    assert { :sourceloc "/Users/schaef/git/jar2bpl/jar2bpl_test/regression/true_positives/tp01/InfeasibleCode01.java",42,31,42,31 } true;
+    temp$436 := temp$335 + 1;
+    assert { :sourceloc "/Users/schaef/git/jar2bpl/jar2bpl_test/regression/true_positives/tp01/InfeasibleCode01.java",42,31,42,31 } true;
+    i31 := temp$436;
+    assert { :sourceloc "/Users/schaef/git/jar2bpl/jar2bpl_test/regression/true_positives/tp01/InfeasibleCode01.java",42,3,44,3 } true;
+    goto block9;
+  block11:
+    assert { :sourceloc "/Users/schaef/git/jar2bpl/jar2bpl_test/regression/true_positives/tp01/InfeasibleCode01.java",42,3,44,3 } true;
+    assert { :sourceloc "/Users/schaef/git/jar2bpl/jar2bpl_test/regression/true_positives/tp01/InfeasibleCode01.java",42,3,44,3 } true;
+    return;
+}
+
+
+implementation void$InfeasibleCode01$infeasible3$1893($this:ref, $in_parameter__0:int, $in_parameter__1:int) returns ($exception:ref){
+    
+var temp$141 : int;    
+var a38 : int;    
+var temp$343 : int;    
+var temp$040 : int;    
+var b39 : int;    
+var temp$545 : int;    
+var temp$444 : int;    
+var temp$242 : int;    
+var this37 : ref;
+    assume { :sourceloc "/Users/schaef/git/jar2bpl/jar2bpl_test/regression/true_positives/tp01/InfeasibleCode01.java",-1,-1,-1,-1 } $this != $null;
+    assert { :sourceloc "/Users/schaef/git/jar2bpl/jar2bpl_test/regression/true_positives/tp01/InfeasibleCode01.java",47,2,52,2 } true;
+    this37 := $this;
+    assert { :sourceloc "/Users/schaef/git/jar2bpl/jar2bpl_test/regression/true_positives/tp01/InfeasibleCode01.java",47,26,47,30 } true;
+    a38 := $in_parameter__0;
+    assert { :sourceloc "/Users/schaef/git/jar2bpl/jar2bpl_test/regression/true_positives/tp01/InfeasibleCode01.java",47,33,47,37 } true;
+    b39 := $in_parameter__1;
+    assert { :sourceloc "/Users/schaef/git/jar2bpl/jar2bpl_test/regression/true_positives/tp01/InfeasibleCode01.java",48,3,48,3 } true;
+    temp$040 := 1;
+    assert { :sourceloc "/Users/schaef/git/jar2bpl/jar2bpl_test/regression/true_positives/tp01/InfeasibleCode01.java",48,3,48,3 } true;
+    b39 := temp$040;
+    assert { :sourceloc "/Users/schaef/git/jar2bpl/jar2bpl_test/regression/true_positives/tp01/InfeasibleCode01.java",49,7,49,9 } true;
+    if (a38 > 0) {
+        assert { :sourceloc "/Users/schaef/git/jar2bpl/jar2bpl_test/regression/true_positives/tp01/InfeasibleCode01.java",49,7,49,9 } { :comment "thenblock" } true;
+        goto block12;
+    } else {
+        assert { :sourceloc "/Users/schaef/git/jar2bpl/jar2bpl_test/regression/true_positives/tp01/InfeasibleCode01.java",49,7,49,9 } { :comment "elseblock" } true;
+    }
+    assert { :sourceloc "/Users/schaef/git/jar2bpl/jar2bpl_test/regression/true_positives/tp01/InfeasibleCode01.java",49,7,49,9 } true;
+    goto block13;
+  block12:
+    assert { :sourceloc "/Users/schaef/git/jar2bpl/jar2bpl_test/regression/true_positives/tp01/InfeasibleCode01.java",49,7,49,9 } true;
+    assert { :sourceloc "/Users/schaef/git/jar2bpl/jar2bpl_test/regression/true_positives/tp01/InfeasibleCode01.java",49,12,49,15 } true;
+    temp$141 := b39;
+    assert { :sourceloc "/Users/schaef/git/jar2bpl/jar2bpl_test/regression/true_positives/tp01/InfeasibleCode01.java",49,12,49,12 } true;
+    temp$242 := temp$141 + -1;
+    assert { :sourceloc "/Users/schaef/git/jar2bpl/jar2bpl_test/regression/true_positives/tp01/InfeasibleCode01.java",49,12,49,12 } true;
+    b39 := temp$242;
+  block13:
+    assert { :sourceloc "/Users/schaef/git/jar2bpl/jar2bpl_test/regression/true_positives/tp01/InfeasibleCode01.java",49,12,49,12 } true;
+    assert { :sourceloc "/Users/schaef/git/jar2bpl/jar2bpl_test/regression/true_positives/tp01/InfeasibleCode01.java",50,3,50,8 } true;
+    assert { :sourceloc "/Users/schaef/git/jar2bpl/jar2bpl_test/regression/true_positives/tp01/InfeasibleCode01.java",50,3,50,8 } b39 != 0;
+    temp$343 := 1 div b39;
+    assert { :sourceloc "/Users/schaef/git/jar2bpl/jar2bpl_test/regression/true_positives/tp01/InfeasibleCode01.java",50,3,50,3 } true;
+    b39 := temp$343;
+    assert { :sourceloc "/Users/schaef/git/jar2bpl/jar2bpl_test/regression/true_positives/tp01/InfeasibleCode01.java",51,7,51,10 } true;
+    if (a38 <= 0) {
+        assert { :sourceloc "/Users/schaef/git/jar2bpl/jar2bpl_test/regression/true_positives/tp01/InfeasibleCode01.java",51,7,51,10 } { :comment "thenblock" } true;
+        goto block14;
+    } else {
+        assert { :sourceloc "/Users/schaef/git/jar2bpl/jar2bpl_test/regression/true_positives/tp01/InfeasibleCode01.java",51,7,51,10 } { :comment "elseblock" } true;
+    }
+    assert { :sourceloc "/Users/schaef/git/jar2bpl/jar2bpl_test/regression/true_positives/tp01/InfeasibleCode01.java",51,7,51,10 } true;
+    goto block15;
+  block14:
+    assert { :sourceloc "/Users/schaef/git/jar2bpl/jar2bpl_test/regression/true_positives/tp01/InfeasibleCode01.java",51,7,51,10 } true;
+    assert { :sourceloc "/Users/schaef/git/jar2bpl/jar2bpl_test/regression/true_positives/tp01/InfeasibleCode01.java",51,13,51,22 } true;
+    temp$444 := 1 - b39;
+    assert { :sourceloc "/Users/schaef/git/jar2bpl/jar2bpl_test/regression/true_positives/tp01/InfeasibleCode01.java",51,13,51,22 } true;
+    assert { :sourceloc "/Users/schaef/git/jar2bpl/jar2bpl_test/regression/true_positives/tp01/InfeasibleCode01.java",51,13,51,22 } temp$444 != 0;
+    temp$545 := 1 div temp$444;
+    assert { :sourceloc "/Users/schaef/git/jar2bpl/jar2bpl_test/regression/true_positives/tp01/InfeasibleCode01.java",51,13,51,13 } true;
+    b39 := temp$545;
+  block15:
+    assert { :sourceloc "/Users/schaef/git/jar2bpl/jar2bpl_test/regression/true_positives/tp01/InfeasibleCode01.java",51,13,51,13 } true;
+    assert { :sourceloc "/Users/schaef/git/jar2bpl/jar2bpl_test/regression/true_positives/tp01/InfeasibleCode01.java",51,13,51,13 } true;
+    return;
+}
+
+
+implementation boolean$InfeasibleCode01$infeasible4$1894($this:ref, $in_parameter__0:ref) returns ($return:int, $exception:ref){
+    
+var o47 : ref;    
+var temp$048 : ref;    
+var temp$351 : int;    
+var temp$250 : int;    
+var this46 : ref;    
+var temp$149 : ref;
+    assume { :sourceloc "/Users/schaef/git/jar2bpl/jar2bpl_test/regression/true_positives/tp01/InfeasibleCode01.java",-1,-1,-1,-1 } $this != $null;
+    assume $heap[$in_parameter__0,$type] <: java.lang.Object;
+    assert { :sourceloc "/Users/schaef/git/jar2bpl/jar2bpl_test/regression/true_positives/tp01/InfeasibleCode01.java",54,2,60,2 } true;
+    this46 := $this;
+    assert { :sourceloc "/Users/schaef/git/jar2bpl/jar2bpl_test/regression/true_positives/tp01/InfeasibleCode01.java",54,29,54,36 } true;
+    o47 := $in_parameter__0;
+    assert { :sourceloc "/Users/schaef/git/jar2bpl/jar2bpl_test/regression/true_positives/tp01/InfeasibleCode01.java",55,3,55,35 } true;
+    temp$048 := java.io.PrintStream$java.lang.System$err237;
+    assert { :sourceloc "/Users/schaef/git/jar2bpl/jar2bpl_test/regression/true_positives/tp01/InfeasibleCode01.java",55,3,55,35 } true;
+    assert { :sourceloc "/Users/schaef/git/jar2bpl/jar2bpl_test/regression/true_positives/tp01/InfeasibleCode01.java",55,3,55,35 } o47 != $null;
+    call temp$149, $exception := java.lang.String$java.lang.Object$toString$44(o47);
+    assert { :sourceloc "/Users/schaef/git/jar2bpl/jar2bpl_test/regression/true_positives/tp01/InfeasibleCode01.java",55,3,55,35 } true;
+    assert { :sourceloc "/Users/schaef/git/jar2bpl/jar2bpl_test/regression/true_positives/tp01/InfeasibleCode01.java",55,3,55,35 } temp$048 != $null;
+    call $exception := void$java.io.PrintStream$println$217(temp$048, temp$149);
+    assert { :sourceloc "/Users/schaef/git/jar2bpl/jar2bpl_test/regression/true_positives/tp01/InfeasibleCode01.java",56,7,56,13 } true;
+    if (o47 == $null) {
+        assert { :sourceloc "/Users/schaef/git/jar2bpl/jar2bpl_test/regression/true_positives/tp01/InfeasibleCode01.java",56,7,56,13 } { :comment "thenblock" } true;
+        goto block16;
+    } else {
+        assert { :sourceloc "/Users/schaef/git/jar2bpl/jar2bpl_test/regression/true_positives/tp01/InfeasibleCode01.java",56,7,56,13 } { :comment "elseblock" } true;
+    }
+    assert { :sourceloc "/Users/schaef/git/jar2bpl/jar2bpl_test/regression/true_positives/tp01/InfeasibleCode01.java",56,7,56,13 } true;
+    goto block17;
+  block16:
+    assert { :sourceloc "/Users/schaef/git/jar2bpl/jar2bpl_test/regression/true_positives/tp01/InfeasibleCode01.java",56,7,56,13 } true;
+    assert { :sourceloc "/Users/schaef/git/jar2bpl/jar2bpl_test/regression/true_positives/tp01/InfeasibleCode01.java",56,7,56,13 } true;
+    temp$250 := 0;
+    assert { :sourceloc "/Users/schaef/git/jar2bpl/jar2bpl_test/regression/true_positives/tp01/InfeasibleCode01.java",57,4,57,16 } true;
+    $return := temp$250;
+    return;
+  block17:
+    assert { :sourceloc "/Users/schaef/git/jar2bpl/jar2bpl_test/regression/true_positives/tp01/InfeasibleCode01.java",57,4,57,16 } true;
+    assert { :sourceloc "/Users/schaef/git/jar2bpl/jar2bpl_test/regression/true_positives/tp01/InfeasibleCode01.java",57,4,57,16 } true;
+    temp$351 := 1;
+    assert { :sourceloc "/Users/schaef/git/jar2bpl/jar2bpl_test/regression/true_positives/tp01/InfeasibleCode01.java",59,3,59,14 } true;
+    $return := temp$351;
+    return;
+}
+
+
+implementation void$InfeasibleCode01$infeasible5$1895($this:ref) returns ($exception:ref){
+    
+var temp$054 : int;    
+var test53 : ref;    
+var $fakelocal_0 : ref;    
+var temp$155 : ref;    
+var this52 : ref;
+    assume { :sourceloc "/Users/schaef/git/jar2bpl/jar2bpl_test/regression/true_positives/tp01/InfeasibleCode01.java",-1,-1,-1,-1 } $this != $null;
+    assert { :sourceloc "/Users/schaef/git/jar2bpl/jar2bpl_test/regression/true_positives/tp01/InfeasibleCode01.java",62,2,67,2 } true;
+    this52 := $this;
+    assert { :sourceloc "/Users/schaef/git/jar2bpl/jar2bpl_test/regression/true_positives/tp01/InfeasibleCode01.java",63,3,63,25 } true;
+    call $fakelocal_0 := $new(java.lang.String);
+    $stringSizeHeap := $stringSizeHeap[$fakelocal_0 := 8];
+    test53 := $fakelocal_0;
+    assert { :sourceloc "/Users/schaef/git/jar2bpl/jar2bpl_test/regression/true_positives/tp01/InfeasibleCode01.java",64,7,64,22 } true;
+    temp$054 := $stringSizeHeap[test53];
+    assert { :sourceloc "/Users/schaef/git/jar2bpl/jar2bpl_test/regression/true_positives/tp01/InfeasibleCode01.java",64,7,64,22 } true;
+    if (temp$054 == 3) {
+        assert { :sourceloc "/Users/schaef/git/jar2bpl/jar2bpl_test/regression/true_positives/tp01/InfeasibleCode01.java",64,7,64,22 } { :comment "thenblock" } true;
+        goto block18;
+    } else {
+        assert { :sourceloc "/Users/schaef/git/jar2bpl/jar2bpl_test/regression/true_positives/tp01/InfeasibleCode01.java",64,7,64,22 } { :comment "elseblock" } true;
+    }
+    assert { :sourceloc "/Users/schaef/git/jar2bpl/jar2bpl_test/regression/true_positives/tp01/InfeasibleCode01.java",64,7,64,22 } true;
+    goto block19;
+  block18:
+    assert { :sourceloc "/Users/schaef/git/jar2bpl/jar2bpl_test/regression/true_positives/tp01/InfeasibleCode01.java",64,7,64,22 } true;
+    assert { :sourceloc "/Users/schaef/git/jar2bpl/jar2bpl_test/regression/true_positives/tp01/InfeasibleCode01.java",65,4,65,37 } true;
+    temp$155 := java.io.PrintStream$java.lang.System$err237;
+    assert { :sourceloc "/Users/schaef/git/jar2bpl/jar2bpl_test/regression/true_positives/tp01/InfeasibleCode01.java",65,4,65,37 } true;
+    assert { :sourceloc "/Users/schaef/git/jar2bpl/jar2bpl_test/regression/true_positives/tp01/InfeasibleCode01.java",65,4,65,37 } temp$155 != $null;
+    call $exception := void$java.io.PrintStream$println$217(temp$155, $StringConst1);
+  block19:
+    assert { :sourceloc "/Users/schaef/git/jar2bpl/jar2bpl_test/regression/true_positives/tp01/InfeasibleCode01.java",65,4,65,37 } true;
+    assert { :sourceloc "/Users/schaef/git/jar2bpl/jar2bpl_test/regression/true_positives/tp01/InfeasibleCode01.java",65,4,65,37 } true;
+    return;
+}
+
+
+implementation int$InfeasibleCode01$infeasible6$1896($this:ref, $in_parameter__0:ref) returns ($return:int, $exception:ref){
+    
+var temp$664 : int;    
+var temp$159 : int;    
+var this56 : ref;    
+var temp$462 : int;    
+var temp$361 : ref;    
+var arr57 : ref;    
+var temp$563 : int;    
+var temp$058 : ref;    
+var temp$260 : int;
+    assume { :sourceloc "/Users/schaef/git/jar2bpl/jar2bpl_test/regression/true_positives/tp01/InfeasibleCode01.java",-1,-1,-1,-1 } $this != $null;
+    assert { :sourceloc "/Users/schaef/git/jar2bpl/jar2bpl_test/regression/true_positives/tp01/InfeasibleCode01.java",69,2,71,2 } true;
+    this56 := $this;
+    assert { :sourceloc "/Users/schaef/git/jar2bpl/jar2bpl_test/regression/true_positives/tp01/InfeasibleCode01.java",69,25,69,33 } true;
+    arr57 := $in_parameter__0;
+    assert { :sourceloc "/Users/schaef/git/jar2bpl/jar2bpl_test/regression/true_positives/tp01/InfeasibleCode01.java",69,25,69,33 } true;
+    temp$058 := arr57;
+    assert { :sourceloc "/Users/schaef/git/jar2bpl/jar2bpl_test/regression/true_positives/tp01/InfeasibleCode01.java",69,25,69,33 } true;
+    temp$159 := -1;
+    assert { :sourceloc "/Users/schaef/git/jar2bpl/jar2bpl_test/regression/true_positives/tp01/InfeasibleCode01.java",69,25,69,33 } true;
+    assert { :sourceloc "/Users/schaef/git/jar2bpl/jar2bpl_test/regression/true_positives/tp01/InfeasibleCode01.java",69,25,69,33 } temp$159 < $arrSizeHeap[temp$058] && temp$159 >= 0;
+    temp$260 := $intArrHeap[temp$058][temp$159];
+    assert { :sourceloc "/Users/schaef/git/jar2bpl/jar2bpl_test/regression/true_positives/tp01/InfeasibleCode01.java",69,25,69,33 } true;
+    temp$361 := arr57;
+    assert { :sourceloc "/Users/schaef/git/jar2bpl/jar2bpl_test/regression/true_positives/tp01/InfeasibleCode01.java",69,25,69,33 } true;
+    assert { :sourceloc "/Users/schaef/git/jar2bpl/jar2bpl_test/regression/true_positives/tp01/InfeasibleCode01.java",69,25,69,33 } arr57 != $null;
+    temp$462 := $arrSizeHeap[arr57];
+    assert { :sourceloc "/Users/schaef/git/jar2bpl/jar2bpl_test/regression/true_positives/tp01/InfeasibleCode01.java",69,25,69,33 } true;
+    assert { :sourceloc "/Users/schaef/git/jar2bpl/jar2bpl_test/regression/true_positives/tp01/InfeasibleCode01.java",69,25,69,33 } temp$462 < $arrSizeHeap[temp$361] && temp$462 >= 0;
+    temp$563 := $intArrHeap[temp$361][temp$462];
+    assert { :sourceloc "/Users/schaef/git/jar2bpl/jar2bpl_test/regression/true_positives/tp01/InfeasibleCode01.java",69,25,69,33 } true;
+    temp$664 := temp$260 + temp$563;
+    assert { :sourceloc "/Users/schaef/git/jar2bpl/jar2bpl_test/regression/true_positives/tp01/InfeasibleCode01.java",70,3,70,35 } true;
+    $return := temp$664;
+    return;
+}
+
+
+implementation void$InfeasibleCode01$infeasible07$1897($this:ref, $in_parameter__0:ref) returns ($exception:ref){
+    
+var end68 : int;    
+var temp$777 : int;    
+var temp$070 : int;    
+var temp$676 : int;    
+var this65 : ref;    
+var repos67 : int;    
+var temp66 : ref;    
+var temp$272 : ref;    
+var temp$575 : int;    
+var temp$171 : int;    
+var j69 : int;    
+var temp$373 : int;    
+var temp$474 : int;    
+var temp$979 : int;    
+var temp$878 : int;
+    assume { :sourceloc "/Users/schaef/git/jar2bpl/jar2bpl_test/regression/true_positives/tp01/InfeasibleCode01.java",-1,-1,-1,-1 } $this != $null;
+    assert { :sourceloc "/Users/schaef/git/jar2bpl/jar2bpl_test/regression/true_positives/tp01/InfeasibleCode01.java",73,2,86,2 } true;
+    this65 := $this;
+    assert { :sourceloc "/Users/schaef/git/jar2bpl/jar2bpl_test/regression/true_positives/tp01/InfeasibleCode01.java",73,27,73,37 } true;
+    temp66 := $in_parameter__0;
+    assert { :sourceloc "/Users/schaef/git/jar2bpl/jar2bpl_test/regression/true_positives/tp01/InfeasibleCode01.java",74,3,74,17 } true;
+    repos67 := -1;
+    assert { :sourceloc "/Users/schaef/git/jar2bpl/jar2bpl_test/regression/true_positives/tp01/InfeasibleCode01.java",75,3,75,15 } true;
+    end68 := -1;
+    assert { :sourceloc "/Users/schaef/git/jar2bpl/jar2bpl_test/regression/true_positives/tp01/InfeasibleCode01.java",76,3,76,14 } true;
+    j69 := end68;
+  block20:
+    assert { :sourceloc "/Users/schaef/git/jar2bpl/jar2bpl_test/regression/true_positives/tp01/InfeasibleCode01.java",77,3,82,43 } true;
+    assert { :sourceloc "/Users/schaef/git/jar2bpl/jar2bpl_test/regression/true_positives/tp01/InfeasibleCode01.java",78,4,78,7 } true;
+    temp$070 := j69;
+    assert { :sourceloc "/Users/schaef/git/jar2bpl/jar2bpl_test/regression/true_positives/tp01/InfeasibleCode01.java",78,4,78,4 } true;
+    temp$171 := temp$070 + 1;
+    assert { :sourceloc "/Users/schaef/git/jar2bpl/jar2bpl_test/regression/true_positives/tp01/InfeasibleCode01.java",78,4,78,4 } true;
+    j69 := temp$171;
+    assert { :sourceloc "/Users/schaef/git/jar2bpl/jar2bpl_test/regression/true_positives/tp01/InfeasibleCode01.java",79,8,79,19 } true;
+    temp$272 := temp66;
+    assert { :sourceloc "/Users/schaef/git/jar2bpl/jar2bpl_test/regression/true_positives/tp01/InfeasibleCode01.java",79,8,79,19 } true;
+    temp$373 := j69;
+    assert { :sourceloc "/Users/schaef/git/jar2bpl/jar2bpl_test/regression/true_positives/tp01/InfeasibleCode01.java",79,8,79,19 } true;
+    assert { :sourceloc "/Users/schaef/git/jar2bpl/jar2bpl_test/regression/true_positives/tp01/InfeasibleCode01.java",79,8,79,19 } temp$373 < $arrSizeHeap[temp$272] && temp$373 >= 0;
+    temp$474 := $intArrHeap[temp$272][temp$373];
+    assert { :sourceloc "/Users/schaef/git/jar2bpl/jar2bpl_test/regression/true_positives/tp01/InfeasibleCode01.java",79,8,79,19 } true;
+    temp$575 := temp$474;
+    assert { :sourceloc "/Users/schaef/git/jar2bpl/jar2bpl_test/regression/true_positives/tp01/InfeasibleCode01.java",79,8,79,19 } true;
+    if (temp$575 == 97) {
+        assert { :sourceloc "/Users/schaef/git/jar2bpl/jar2bpl_test/regression/true_positives/tp01/InfeasibleCode01.java",79,8,79,19 } { :comment "thenblock" } true;
+        goto block21;
+    } else {
+        assert { :sourceloc "/Users/schaef/git/jar2bpl/jar2bpl_test/regression/true_positives/tp01/InfeasibleCode01.java",79,8,79,19 } { :comment "elseblock" } true;
+    }
+    assert { :sourceloc "/Users/schaef/git/jar2bpl/jar2bpl_test/regression/true_positives/tp01/InfeasibleCode01.java",79,8,79,19 } true;
+    goto block22;
+  block21:
+    assert { :sourceloc "/Users/schaef/git/jar2bpl/jar2bpl_test/regression/true_positives/tp01/InfeasibleCode01.java",79,8,79,19 } true;
+    assert { :sourceloc "/Users/schaef/git/jar2bpl/jar2bpl_test/regression/true_positives/tp01/InfeasibleCode01.java",80,5,80,24 } true;
+    temp$676 := j69 - end68;
+    assert { :sourceloc "/Users/schaef/git/jar2bpl/jar2bpl_test/regression/true_positives/tp01/InfeasibleCode01.java",80,5,80,24 } true;
+    temp$777 := temp$676 - 1;
+    assert { :sourceloc "/Users/schaef/git/jar2bpl/jar2bpl_test/regression/true_positives/tp01/InfeasibleCode01.java",80,5,80,9 } true;
+    repos67 := temp$777;
+  block22:
+    assert { :sourceloc "/Users/schaef/git/jar2bpl/jar2bpl_test/regression/true_positives/tp01/InfeasibleCode01.java",80,5,80,9 } true;
+    assert { :sourceloc "/Users/schaef/git/jar2bpl/jar2bpl_test/regression/true_positives/tp01/InfeasibleCode01.java",80,5,80,9 } true;
+    assert { :sourceloc "/Users/schaef/git/jar2bpl/jar2bpl_test/regression/true_positives/tp01/InfeasibleCode01.java",82,12,82,22 } true;
+    if (repos67 == -1) {
+        assert { :sourceloc "/Users/schaef/git/jar2bpl/jar2bpl_test/regression/true_positives/tp01/InfeasibleCode01.java",82,12,82,22 } { :clone } { :comment "thenblock" } true;
+        goto block23;
+    } else {
+        assert { :sourceloc "/Users/schaef/git/jar2bpl/jar2bpl_test/regression/true_positives/tp01/InfeasibleCode01.java",82,12,82,22 } { :clone } { :comment "elseblock" } true;
+    }
+    assert { :sourceloc "/Users/schaef/git/jar2bpl/jar2bpl_test/regression/true_positives/tp01/InfeasibleCode01.java",82,12,82,22 } true;
+    goto block24;
+  block23:
+    assert { :sourceloc "/Users/schaef/git/jar2bpl/jar2bpl_test/regression/true_positives/tp01/InfeasibleCode01.java",82,12,82,22 } true;
+    assert { :sourceloc "/Users/schaef/git/jar2bpl/jar2bpl_test/regression/true_positives/tp01/InfeasibleCode01.java",82,27,82,41 } true;
+    assert { :sourceloc "/Users/schaef/git/jar2bpl/jar2bpl_test/regression/true_positives/tp01/InfeasibleCode01.java",82,27,82,41 } temp66 != $null;
+    temp$878 := $arrSizeHeap[temp66];
+    assert { :sourceloc "/Users/schaef/git/jar2bpl/jar2bpl_test/regression/true_positives/tp01/InfeasibleCode01.java",82,27,82,41 } true;
+    if (j69 < temp$878) {
+        assert { :sourceloc "/Users/schaef/git/jar2bpl/jar2bpl_test/regression/true_positives/tp01/InfeasibleCode01.java",82,27,82,41 } { :comment "thenblock" } true;
+        goto block20;
+    } else {
+        assert { :sourceloc "/Users/schaef/git/jar2bpl/jar2bpl_test/regression/true_positives/tp01/InfeasibleCode01.java",82,27,82,41 } { :comment "elseblock" } true;
+    }
+    assert { :sourceloc "/Users/schaef/git/jar2bpl/jar2bpl_test/regression/true_positives/tp01/InfeasibleCode01.java",82,27,82,41 } true;
+    goto block24;
+    assert { :sourceloc "/Users/schaef/git/jar2bpl/jar2bpl_test/regression/true_positives/tp01/InfeasibleCode01.java",82,27,82,41 } true;
+    goto block20;
+  block24:
+    assert { :sourceloc "/Users/schaef/git/jar2bpl/jar2bpl_test/regression/true_positives/tp01/InfeasibleCode01.java",82,27,82,41 } true;
+    assert { :sourceloc "/Users/schaef/git/jar2bpl/jar2bpl_test/regression/true_positives/tp01/InfeasibleCode01.java",83,7,83,17 } true;
+    if (repos67 == -1) {
+        assert { :sourceloc "/Users/schaef/git/jar2bpl/jar2bpl_test/regression/true_positives/tp01/InfeasibleCode01.java",83,7,83,17 } { :clone } { :comment "thenblock" } true;
+        goto block25;
+    } else {
+        assert { :sourceloc "/Users/schaef/git/jar2bpl/jar2bpl_test/regression/true_positives/tp01/InfeasibleCode01.java",83,7,83,17 } { :clone } { :comment "elseblock" } true;
+    }
+    assert { :sourceloc "/Users/schaef/git/jar2bpl/jar2bpl_test/regression/true_positives/tp01/InfeasibleCode01.java",83,7,83,17 } true;
+    goto block26;
+  block25:
+    assert { :sourceloc "/Users/schaef/git/jar2bpl/jar2bpl_test/regression/true_positives/tp01/InfeasibleCode01.java",83,7,83,17 } true;
+    assert { :sourceloc "/Users/schaef/git/jar2bpl/jar2bpl_test/regression/true_positives/tp01/InfeasibleCode01.java",84,4,84,8 } true;
+    temp$979 := 0;
+    assert { :sourceloc "/Users/schaef/git/jar2bpl/jar2bpl_test/regression/true_positives/tp01/InfeasibleCode01.java",84,4,84,8 } true;
+    repos67 := temp$979;
+  block26:
+    assert { :sourceloc "/Users/schaef/git/jar2bpl/jar2bpl_test/regression/true_positives/tp01/InfeasibleCode01.java",84,4,84,8 } true;
+    assert { :sourceloc "/Users/schaef/git/jar2bpl/jar2bpl_test/regression/true_positives/tp01/InfeasibleCode01.java",84,4,84,8 } true;
+    return;
+}
+
+
+implementation void$InfeasibleCode01$$la$init$ra$$1898($this:ref) returns ($exception:ref){
+    
+var this80 : ref;
+    assume { :sourceloc "/Users/schaef/git/jar2bpl/jar2bpl_test/regression/true_positives/tp01/InfeasibleCode01.java",-1,-1,-1,-1 } $this != $null;
+    assert { :sourceloc "/Users/schaef/git/jar2bpl/jar2bpl_test/regression/true_positives/tp01/InfeasibleCode01.java",7,-1,-1,-1 } true;
+    this80 := $this;
+    assert { :sourceloc "/Users/schaef/git/jar2bpl/jar2bpl_test/regression/true_positives/tp01/InfeasibleCode01.java",7,-1,-1,-1 } true;
+    call $exception := void$java.lang.Object$$la$init$ra$$38(this80);
+    assert { :sourceloc "/Users/schaef/git/jar2bpl/jar2bpl_test/regression/true_positives/tp01/InfeasibleCode01.java",7,-1,-1,-1 } true;
+    return;
+}
+
+
